### 重要的性质
$$gcd(x+y,lcm(x,y))=gcd(x,y)$$
理由：
$$gcd(x,y)=k,则gcd(\frac{x}{k},\frac{y}{k})=1,记x_0=\frac{x}{k},y_0=\frac{y}{k},即gcd(x_0,y_0)=1. \\
\because gcd(x+y,x)=gcd(x,y) \\
\therefore gcd(x_0+y_0,x_0)=gcd(x_0,y_0)=1 \quad gcd(x_0+y_0,y_0)=gcd(x_0,y_0)=1 \\
令gcd(x_0+y_0,x_0y_0)=c \\
则c \mid (x_0+y_0),c \mid x_0y_0. \\
\because gcd(x_0,y_0)=1 \quad \therefore 要不c \mid x_0，要不c \mid y_0.
\therefore 要不c | gcd(x_0+y_0,x_0) 要不 c | gcd(x_0+y_0,y_0). \\
即 要不c | 1 要不 c | 1. \\
即 c|1. \quad \therefore c=1\\
gcd(x_0+y_0,x_0y_0)=1.\\
x+y=k(x_0+y_0) \\
lcm(x,y)=\frac{xy}{gcd(x,y)}=\frac{k^2x_0y_0}{k}=kx_0y_0 \\
gcd(x+y,lcm(x,y))=gcd(k(x_0+y_0), kx_0y_0)=k\times gcd(x_0+y_0,x_0y_0)=k=gcd(x,y).
$$

因此
$$k=gcd(a,b), \\
xy=k^2x_0y_0=bk\\
x+y=a.$$
注意k是由已知数a,b直接求得的，也是已知数，直接解方程即可。

